Simu/Sep.v
@@ -1,0 +1,323 @@
+Require Import common.Separation.
+Require Import common.Values.
+Require Import common.Errors.
+Require Import cfrontend.Ctypes.
+Require Import lib.Maps.
+Require Import lib.Coqlib.
+
+Require Import Rustre.Common.
+Require Import Syn Sem.
+
+Require Import List.
+Require Import ZArith.BinInt.
+
+Open Scope list.
+Open Scope sep_scope.
+Open Scope Z.
+
+Lemma storev_rule':
+  forall chunk m m' b ofs v (spec1 spec: val -> Prop) P,
+    m |= contains chunk b ofs spec1 ** P ->
+    spec (Val.load_result chunk v) ->
+    Memory.Mem.storev chunk m (Vptr b (Integers.Int.repr ofs)) v = Some m' ->
+    m' |= contains chunk b ofs spec ** P.
+Proof.
+  intros ** Hm Hspec Hstore.
+  apply storev_rule with (1:=Hm) in Hspec.
+  destruct Hspec as [m'' [Hmem Hspec]].
+  rewrite Hmem in Hstore. injection Hstore.
+  intro; subst. assumption.
+Qed.
+
+(* Introduce sepall *)
+
+Program Definition sepemp: massert :=  pure True.
+
+Lemma sepemp_disjoint:
+  forall P, disjoint_footprint P sepemp.
+Proof.
+  unfold disjoint_footprint. auto.
+Qed.
+
+Lemma sepemp_right:
+  forall P,
+    massert_eqv P (P ** sepemp).
+Proof.
+  split; split; simpl; try (auto using sepemp_disjoint); intuition.
+Qed.
+
+Lemma sepemp_left:
+  forall P,
+    massert_eqv P (sepemp ** P).
+Proof.
+  intros. rewrite sep_comm. rewrite <-sepemp_right. reflexivity.
+Qed.
+
+Program Definition sepfalse: massert := {| m_pred := fun m => False;
+                                            m_footprint := fun b ofs => True |}.
+Next Obligation.
+  contradiction.
+Defined.
+
+Section Sepall.
+  Context {A: Type}.
+
+  Fixpoint sepall (p: A -> massert) (xs: list A) : massert :=
+    match xs with
+    | nil => sepemp
+    | x::xs => p x ** sepall p xs
+    end.
+
+  Lemma sepall_cons:
+    forall p x xs,
+      massert_eqv (sepall p (x::xs))
+                  (p x ** sepall p xs).
+  Proof.
+    constructor; constructor; trivial.
+  Qed.
+
+  Lemma sepall_app:
+    forall p xs ys,
+      massert_eqv (sepall p (xs ++ ys))
+                  (sepall p xs ** sepall p ys).
+  Proof.
+    induction xs.
+    - intros. 
+      rewrite sep_comm.
+      rewrite <-sepemp_right.
+      reflexivity.
+    - intros.
+      simpl.
+      rewrite sep_assoc.
+      rewrite IHxs.
+      reflexivity.
+  Qed.
+
+  Lemma sepall_breakout:
+    forall ys ws x xs p,
+      ys = ws ++ x :: xs ->
+      massert_eqv (sepall p ys) (p x ** sepall p (ws ++ xs)).
+  Proof.
+    intros ** Hys.
+    rewrite sepall_app.
+    rewrite sep_swap.
+    rewrite <-sepall_cons.
+    rewrite <-sepall_app.
+    rewrite <-Hys.
+    reflexivity.
+  Qed.
+
+  Lemma sepall_in:
+    forall x ys,
+      In x ys ->
+      exists ws xs,
+        ys = ws ++ x :: xs
+        /\ (forall p,
+               massert_eqv (sepall p ys)
+                           (p x ** sepall p (ws ++ xs))).
+  Proof.
+    intros x ys Hin.
+    apply in_split in Hin.
+    destruct Hin as [ws [xs Hys]].
+    exists ws, xs.
+    split; auto. 
+    intro p. apply sepall_breakout with (1:=Hys).
+  Qed.
+
+  Lemma sepall_sepfalse:
+    forall m p xs,
+      m |= sepall p xs ->
+      (forall x, In x xs -> p x <> sepfalse).
+  Proof.
+    intros m p xs Hall x Hin Hp.
+    apply sepall_in in Hin.
+    destruct Hin as [ws [ys [Hys Heq]]].
+    rewrite Heq in Hall.
+    apply sep_comm in Hall.
+    apply sep_drop in Hall.
+    rewrite Hp in Hall.
+    destruct Hall.
+  Qed.
+
+  Lemma sepall_switchp:
+    forall f f' xs,
+      List.NoDup xs ->
+      (forall x, In x xs -> f x = f' x) ->
+      massert_eqv (sepall f xs) (sepall f' xs).
+  Proof.
+    induction xs as [|x xs IH].
+    reflexivity.
+    intros Hdup Hin.
+    inversion_clear Hdup.
+    repeat rewrite sepall_cons.
+    rewrite Hin; [|now apply in_eq].
+    rewrite IH; [reflexivity|assumption|].
+    intros; apply Hin. constructor (assumption).
+  Qed.
+
+End Sepall.
+
+Section SplitRange.
+  Variable env: composite_env.
+  Variable id: ident.
+  Variable co: composite.
+
+  Hypothesis Henv: Ctypes.composite_env_consistent env.
+  Hypothesis Hco: env!id = Some co.
+  Hypothesis Hstruct: co_su co = Struct.
+
+  Lemma split_range_fields':
+    forall b lo,
+      NoDupMembers (co_members co) ->
+      massert_imp (range b lo (lo + sizeof_struct env 0 (co_members co)))
+                  (sepall (fun (fld: ident * type) =>
+                             let (id, ty) := fld in
+                             match field_offset env id (co_members co) with
+                             | OK ofs  => range b (lo + ofs) (lo + ofs + sizeof env ty)
+                             | Error _ => sepfalse
+                             end) (co_members co)).
+  Proof.
+    intros b lo Hndup.
+    cut (forall cur,
+            massert_imp
+              (range b (lo + cur)
+                       (lo + sizeof_struct env cur (co_members co)))
+              (sepall (fun fld : ident * type =>
+                         let (id0, ty) := fld in
+                         match field_offset_rec env id0 (co_members co) cur with
+                         | OK ofs => range b (lo + ofs) (lo + ofs + sizeof env ty)
+                         | Error _ => sepfalse
+                         end) (co_members co))).
+    - intro HH.
+      specialize HH with 0. rewrite Z.add_0_r in HH.
+      apply HH.
+    - induction (co_members co) as [|x xs IH]; [now constructor|].
+      destruct x as [id' ty'].
+      apply nodupmembers_cons in Hndup.
+      destruct Hndup as [Hnin Hndup].
+      specialize (IH Hndup).
+      intro cur.
+      Opaque sepconj. simpl.
+      rewrite peq_true.
+      erewrite sepall_switchp.
+      2:now apply NoDupMembers_NoDup.
+      + rewrite range_split'
+        with (mid:=lo + (align cur (alignof env ty') + sizeof env ty')).
+        * apply sep_imp'.
+          2:now apply IH.
+          rewrite range_split'
+          with (mid:=lo + align cur (alignof env ty')).
+          rewrite sep_drop. rewrite Z.add_assoc. reflexivity.
+          split.
+          now apply Z.add_le_mono_l; apply align_le; apply alignof_pos.
+          apply Z.add_le_mono_l.
+          rewrite <-Z.add_0_r at 1. apply Z.add_le_mono_l.
+          apply Z.ge_le. apply sizeof_pos.
+        * split.
+          2:now apply Z.add_le_mono_l; apply sizeof_struct_incr.
+          apply Z.add_le_mono_l.
+          rewrite <-Z.add_0_r at 1. apply Z.add_le_mono.
+          apply align_le. apply alignof_pos.
+          apply Z.ge_le. apply sizeof_pos.
+      + intros fld Hin.
+        destruct fld.
+        rewrite peq_false.
+        reflexivity.
+        intro Heq; subst.
+        apply Hnin.
+        eapply In_InMembers; eassumption.
+  Qed.
+
+  (* A useful lemma for accessing a struct through its fields. It is an
+     implication rather than an equivalence since information about
+     inter-field padding is lost. It is thus not possible to recover the
+     range from the sepall, which may inhibit reasoning about By_copy
+     assignments of complete records. *)
+  Lemma split_range_fields:
+    forall b lo,
+      NoDupMembers (co_members co) ->
+      massert_imp (range b lo (lo + co_sizeof co))
+                  (sepall (fun (fld: ident * type) =>
+                      let (id, ty) := fld in
+                      match field_offset env id (co_members co) with
+                      | OK ofs  => range b (lo + ofs) (lo + ofs + sizeof env ty)
+                      | Error _ => sepfalse
+                      end) (co_members co)).
+  Proof.
+    intros b lo Hndup.
+    apply Henv in Hco.
+    rewrite (co_consistent_sizeof _ _ Hco).
+    rewrite (co_consistent_alignof _ _ Hco).
+    rewrite Hstruct.
+    simpl.
+    rewrite range_split'
+    with (mid:=lo + sizeof_struct env 0 (co_members co)).
+    - rewrite sep_comm. rewrite sep_drop.
+      apply split_range_fields' with (1:=Hndup).
+    - split.
+      * rewrite <-Z.add_0_r at 1.
+        apply Z.add_le_mono_l.
+        apply sizeof_struct_incr.
+      * apply Z.add_le_mono_l.
+        apply align_le.
+        apply alignof_composite_pos.
+  Qed.
+
+End SplitRange.
+
+Section Staterep.
+  Variable ge : composite_env.
+
+  Fixpoint staterep (p: program) (clsnm: ident) (me: menv)
+                    (b: block) (ofs: Z) : massert :=
+    match p with
+    | nil => sepfalse
+    | cls::p' =>
+      if ident_eqb clsnm cls.(c_name)
+      then
+        sepall (fun (xty: ident * typ) =>
+                  let (x, ty) := xty in
+                  match field_offset ge x (make_members cls) with
+                  | OK d =>
+	            Separation.contains (chunk_of_type ty) b (ofs + d)
+                                        (match_value x me.(mm_values))
+                  | Error _ => sepfalse
+                  end) cls.(c_mems)
+        **
+        sepall (fun (o: obj_dec) =>
+                  let i := obj_inst o in
+                  match field_offset ge i (make_members cls) with
+                  | OK d =>
+                    staterep p' o.(obj_class) (instance_match i me) b (ofs + d)
+                  | Error _ => sepfalse
+                  end) cls.(c_objs)
+      else staterep p' clsnm me b ofs
+    end.
+
+  Lemma staterep_skip_cons:
+    forall cls prog clsnm me b ofs,
+      clsnm <> cls.(c_name) ->
+      massert_eqv (staterep (cls::prog) clsnm me b ofs)
+                  (staterep prog clsnm me b ofs).
+  Proof.
+    intros ** Hnm.
+    apply ident_eqb_neq in Hnm.
+    simpl; rewrite Hnm.
+    reflexivity.
+  Qed.
+
+  Lemma staterep_skip_app:
+    forall clsnm prog oprog me b ofs,
+      ~ClassIn clsnm oprog ->
+      massert_eqv (staterep (oprog ++ prog) clsnm me b ofs)
+                  (staterep prog clsnm me b ofs).
+  Proof.
+    intros ** Hnin.
+    induction oprog as [|cls oprog IH].
+    - rewrite app_nil_l. reflexivity.
+    - apply NotClassIn in Hnin. destruct Hnin.
+      rewrite <-app_comm_cons.
+      rewrite staterep_skip_cons; auto.
+  Qed.
+
+End Staterep.
